finish specs for waitfreestack proof

Examples/WaitFreeStackSpec.v
@@ -18,6 +18,161 @@ Variant WaitFreeStackSig {A} : ESig :=
 | WFPop : WaitFreeStackSig (StkRet (option A)).
 Arguments WaitFreeStackSig : clear implicits.
 
+Module AtomicWFStack.
+  Variant WFStackState {T V} :=
+  | WFSsIdle (vs : list V)
+  | WFSsPend (t : Name T) (vs : list V) {R:Type} (m:WaitFreeStackSig V R).
+  Arguments WFStackState : clear implicits.
+
+  Definition eval_stack {T V} (st : WFStackState T V) : list V :=
+    match st with
+    | WFSsIdle vs | WFSsPend _ vs _ => vs
+    end.
+
+  Variant WFStackStep {T A} : WFStackState T A -> ThreadEvent T (WaitFreeStackSig A) -> WFStackState T A -> Prop :=
+  | WFCall vs i R (m : _ R):
+      WFStackStep (WFSsIdle vs) (i, CallEv m) (WFSsPend i vs m)
+  | WFRetFail vs i R (m : _ (StkRet R)):
+      WFStackStep
+        (WFSsPend i vs m)
+        (i, RetEv m FAIL)
+        (WFSsIdle vs)
+  | WFPushRetSucc i v vs :
+      WFStackStep
+        (WFSsPend i vs (WFPush v))
+        (i, RetEv (WFPush v) (PASS tt))
+        (WFSsIdle (v :: vs))
+  | WFPopRetSome i v vs :
+      WFStackStep
+        (WFSsPend i (v :: vs) WFPop)
+        (i, RetEv WFPop (PASS (Some v)))
+        (WFSsIdle vs)
+  | WFPopRetNone i :
+      WFStackStep
+        (WFSsPend i nil WFPop)
+        (i, RetEv WFPop (PASS None))
+        (WFSsIdle nil).
+
+  Require Import Coq.Lists.List.
+  Import ListNotations.
+  Lemma double_ind {A} :
+    forall (P : list A -> Prop),
+    P [] ->
+    (forall x, P [x]) ->
+    (forall x y xs, P xs -> P (x :: y :: xs)) ->
+    forall xs,
+    P xs.
+    intros.
+    generalize dependent xs.
+    fix rec 1.
+    intros.
+    destruct xs.
+    { apply H. }
+    destruct xs.
+    { apply H0. }
+    {
+      apply H1.
+      apply rec.
+    }
+  Qed.
+
+  Program Definition WFStackSpec {T A} : Spec T (WaitFreeStackSig A) := {|
+    State := WFStackState T A;
+    Step := WFStackStep;
+    Init := WFSsIdle nil
+  |}.
+  Next Obligation.
+    generalize dependent (@nil A).
+    apply double_ind with
+      (P := fun p => forall l, Steps WFStackStep (WFSsIdle l) p s -> SeqConsistent (fun _ : Name T => None) p); intros; try constructor.
+    {
+      inversion H; subst.
+      inversion H2; subst.
+      eapply SCCall with
+        (a':=fun j =>
+          if i =? j then
+            Some (existT _ _ _)
+          else
+            None);
+      [auto|
+      now rewrite eqb_id|
+      apply differ_pointwise_trivial| ].
+      constructor.
+    }
+    {
+      inversion H0; subst; clear H0.
+      inversion H3; subst; clear H3.
+      inversion H5; subst; clear H5.
+      inversion H2; subst; clear H2;
+        (eapply SCCall with
+          (a':=fun j =>
+          if i =? j then
+            Some (existT _ _ _)
+          else
+            None);
+        [auto|
+        now rewrite eqb_id|
+        apply differ_pointwise_trivial| ];
+        eapply SCRet with (a':=fun j => None); [
+          now rewrite eqb_id|
+          auto|
+          unfold differ_pointwise; intros; erewrite eqb_nid; eauto|
+          eauto
+        ]).
+    }
+  Defined.
+    (* remember (WFSsIdle nil) as st.
+    remember (fun _ : Name T => None) as tst.
+    assert (forall tid, tst tid <> None <-> exists vs, st = WFSsPend tid vs) as Hinv;
+    [split; intros; subst; [|destruct H0]; congruence|].    
+    clear Heqst. clear Heqtst.
+    generalize dependent tst.
+    generalize dependent st.
+    induction p; [constructor|];intros.
+    destruct a as [i ev].
+    inversion H; subst.
+    inversion H2; subst.
+    {
+      assert (forall j, tst j = None).
+      {
+        intros.
+        specialize (Hinv j) as [? _].
+        destruct (tst j); auto.
+        assert (exists vs0 : list A, WFSsIdle vs = WFSsPend j vs0) as [? ?];
+        [apply H0; inversion 1|].
+        inversion H1.
+      }
+
+      eapply SCCall with
+        (a':=fun j =>
+        if i =? j then
+          Some (existT _ _ _)
+        else
+          tst j).
+      - apply H0.
+      - rewrite eqb_id; constructor.
+      - apply differ_pointwise_trivial.
+      - apply (IHp (WFSsPend i vs)); auto.
+        split; intros.
+        + destruct (i =? tid) eqn:eq; try congruence.
+          rewrite eqb_iff in eq; subst.
+          eauto.
+        + destruct H1.
+          inversion H1; subst.
+          rewrite eqb_id; intros; congruence.
+    }
+    {
+      apply SCRet with (a':=fun j => None); auto.
+
+    } *)
+End AtomicWFStack.
+
+Module SetWFStack.
+  
+End SetWFStack.
+
+
+
 Record WaitFreeStackPend {T A} := MkWFSPend {
   StkRetTy : Type;
   StkName : Name T;
