Examples/MemSpec.v
@@ -1,0 +1,151 @@
+From LHL.Core Require Import
+  Program
+  Specs
+  Logic.
+
+From LHL.Util Require Import
+  Tactics
+  TransUtil
+  Util.
+
+Require Import Coq.Logic.FunctionalExtensionality.
+
+Definition Addr := nat.
+
+Variant MemSig {V} : ESig :=
+| MAlloc : MemSig Addr
+| MWrite (addr : Addr) (val : V) : MemSig unit
+| MRead (addr : Addr) : MemSig V.
+Arguments MemSig : clear implicits.
+
+Definition Heap {V : Type} : Type := Addr -> option V.
+Definition heap_update {V : Type} (addr : Addr) (val : V) (h : Heap) : Heap :=
+  fun addr' => if Nat.eqb addr addr' then Some val else h addr'.
+Definition empty_heap {V : Type} : Heap := fun _ => @None V.
+
+Module WriteRacyMem.
+  Variant MemState {T V} :=
+  | MsIdle (heap : @Heap V)
+  | MsAllocPend (t : Name T) (heap : @Heap V)
+  | MsReadPend (t : Name T) (heap : @Heap V) (addr : Addr)
+  | MsWritePend (t : Name T) (heap : @Heap V) (addr : Addr) (val : V)
+  | MsUBIdle
+  | MsUBPend (t : Name T) {R : Type} (m : MemSig V R)
+  | MsUBWritePend (t : Name T) {R : Type} (m : MemSig V R)
+                  (t' : Name T) {R' : Type} (m' : MemSig V R').
+  Arguments MemState : clear implicits.
+
+  Definition eval_heap {T V} (st : MemState T V) : option (@Heap V) :=
+    match st with
+    | MsIdle h | MsAllocPend _ h | MsReadPend _ h _ | MsWritePend _ h _ _ => Some h
+    | _ => None
+    end.
+
+  Variant MemStep {T V} : MemState T V -> (ThreadEvent T (MemSig V)) -> MemState T V -> Prop :=
+    (* alloc steps *)
+    | MemMAllocCall i h:
+      MemStep (MsIdle h) (i, CallEv MAlloc) (MsAllocPend i h)
+    | MemMAllocRet i h (v:V) (l:Addr):
+      (* allocate a new location *)
+      h l = None ->
+      MemStep (MsAllocPend i h)
+              (i, RetEv MAlloc l) 
+              (* instantiate the location with some arbitrary value *)
+              (MsIdle (heap_update l v h))
+    (* read steps *)
+    | MemReadCall i h l:
+      MemStep (MsIdle h) (i, CallEv (MRead l)) (MsReadPend i h l)
+    | MemReadRet i h l v:
+      (* can only read locations that are ready *)
+      (* read pending values is undefined because the spec needs to ensure this will never happen *)
+      h l = Some v ->
+      MemStep (MsReadPend i h l) (i, RetEv (MRead l) v) (MsIdle h)
+    | MemReadUndefined i h l v:
+      (* read undefined locations cause UB *)
+      h l = None ->
+      (* read value is random *)
+      MemStep (MsReadPend i h l) (i, RetEv (MRead l) v) MsUBIdle
+    (* write steps *)
+    | MemWriteCall i h l v:
+      MemStep (MsIdle h)
+              (i, CallEv (MWrite l v))
+              (MsWritePend i h l v)
+    | MemWriteCallRace i h l v j v':
+      i <> j ->
+      MemStep (MsWritePend j h l v')
+              (i, CallEv (MWrite l v))
+              (MsUBWritePend j (MWrite l v') i (MWrite l v))
+    | MemWriteRetUndef i h l v:
+      h l = None ->
+      MemStep (MsWritePend i h l v) (i, RetEv (MWrite l v) tt) MsUBIdle
+    | MemWriteRet i h l v v':
+      h l = Some v' ->
+      MemStep (MsWritePend i h l v)
+              (i, RetEv (MWrite l v) tt)
+              (* update the location to ready value after return *)
+              (MsIdle (heap_update l v h))
+    (* UB steps *)
+    | MemStepUBCall i R (m : MemSig _ R):
+      MemStep MsUBIdle (i, CallEv m) (MsUBPend i m)
+    | MemStepUBRet i R (m : MemSig _ R) v:
+      MemStep (MsUBPend i m) (i, RetEv m v) MsUBIdle
+    | MemStepUBWriteRet i R (m : MemSig _ R) v j R' (m' : MemSig _ R'):
+      i <> j ->
+      MemStep (MsUBWritePend i m j m') (i, RetEv m v) (MsUBPend j m').
+  Arguments MemStep : clear implicits.
+
+  Definition mst2tst {T V} (st : MemState T V) (i : Name T) : option {R : Type & MemSig V R} :=
+    match st with
+    | MsIdle _ | MsUBIdle => None
+    | MsAllocPend j _ =>
+        if i =? j then Some (existT _ _ MAlloc) else None
+    | MsReadPend j _ l =>
+        if i =? j then Some (existT _ _ (MRead l)) else None
+    | MsWritePend j _ l v =>
+        if i =? j then Some (existT _ _ (MWrite l v)) else None
+    | MsUBPend j m => 
+        if i =? j then Some (existT _ _ m) else None
+    | MsUBWritePend j1 m1 j2 m2 => 
+        if i =? j1 then Some (existT _ _ m1) else
+          if i =? j2 then Some (existT _ _ m2) else None
+    end.
+
+
+  Program Definition memSpec {T A} : Spec T (MemSig A) := {|
+    State := MemState T A;
+    Step := MemStep T A;
+    Init := MsIdle empty_heap
+  |}.
+  Next Obligation.
+    remember (fun _ : Name T => None) as tst.
+    remember (MsIdle empty_heap) as mst.
+    assert (tst = mst2tst mst);
+    [apply functional_extensionality; intros; subst; auto|].
+    rewrite H0.
+    clear dependent tst.
+    clear Heqmst.
+
+    generalize dependent mst.
+    induction p; intros; try constructor.
+
+    inversion H; subst; clear H.
+    inversion H2; subst;
+    try (eapply SCCall; eauto;
+    [simpl; rewrite eqb_id; auto|]);
+    try (eapply SCRet; eauto;
+    [simpl; rewrite eqb_id; auto|
+    simpl; auto|]);
+    try (unfold differ_pointwise; simpl;
+    intros ? Hineq; apply eqb_nid in Hineq; now rewrite Hineq).
+    {
+      eapply SCCall with (a' := mst2tst (MsUBWritePend j (MWrite l v') i (MWrite l v))); simpl; auto.
+      - apply eqb_nid in H; now rewrite H.
+      - apply eqb_nid in H; rewrite H; now rewrite eqb_id.
+      - unfold differ_pointwise; simpl; intros.
+        apply eqb_nid in H0; now rewrite H0.
+    }
+    {
+      apply eqb_nid in H; now rewrite H.
+    }
+  Defined.
+End WriteRacyMem.
